DS/Deque.v
@@ -2,6 +2,8 @@ Add Rec LoadPath "/home/zeimer/Code/Coq".
 
 Require Import RCCBase.
 
+Set Implicit Arguments.
+
 Definition Deque (A : Type) : Type := list A * list A.
 
 (* Auxiliary function that restores balance. *)
@@ -20,11 +22,8 @@ Definition halve {A : Type} (l : list A) : list A * list A :=
 
 Function deque {A : Type} (f r : list A) : Deque A :=
 match f, r with
-    | [], [] => (f, r)
-    | [], [_] => (f, r)
-    | [], _ => let '(r, f) := halve r in (rev f, r)
-    | [_], [] => (f, r)
-    | _, [] => let '(f, r) := halve f in (f, rev r)
+    | [], _ :: _ :: _ => let '(r, f) := halve r in (rev f, r)
+    | _ :: _ :: _, [] => let '(f, r) := halve f in (f, rev r)
     | _, _ => (f, r)
 end.
 
@@ -42,18 +41,16 @@ Definition cons {A : Type} (x : A) (d : Deque A) : Deque A :=
 
 Function head {A : Type} (d : Deque A) : option A :=
 match d with
-    | ([], []) => None
+    | (h :: _, _) => Some h
     | ([], [h]) => Some h
     | ([], _) => None
-    | (h :: _, _) => Some h
 end.
 
 Function tail {A : Type} (d : Deque A) : option (Deque A) :=
 match d with
-    | ([], []) => None
+    | (_ :: t, r) => Some (deque t r)
     | ([], [_]) => Some empty
     | ([], _) => None
-    | (_ :: t, r) => Some (deque t r)
 end.
 
 Definition snoc {A : Type} (x : A) (d : Deque A) : Deque A :=
@@ -61,23 +58,21 @@ Definition snoc {A : Type} (x : A) (d : Deque A) : Deque A :=
 
 Function last {A : Type} (d : Deque A) : option A :=
 match d with
-    | ([], []) => None
+    | (_, x :: _) => Some x
     | ([x], []) => Some x
     | (_, []) => None
-    | (_, x :: _) => Some x
 end.
 
 Function init {A : Type} (d : Deque A) : option (Deque A) :=
 match d with
-    | ([], []) => None
+    | (f, _ :: t) => Some (deque f t)
     | ([_], []) => Some empty
     | (_, []) => None
-    | (f, _ :: t) => Some (deque f t)
 end.
 
 (** Lemmas for [split]. *)
 Lemma split_inv_l :
-  forall (A : Type) (n : nat) (l r : list A),
+  forall {A : Type} {n : nat} {l r : list A},
     split n l = ([], r) -> n = 0 \/ (l = [] /\ r = []).
 Proof.
   intros. functional induction @split A n l.
@@ -87,7 +82,7 @@ Proof.
 Qed.
 
 Lemma split_inv_r :
-  forall (A : Type) (n : nat) (l f : list A),
+  forall {A : Type} {n : nat} {l f : list A},
     split n l = (f, []) -> length l <= n \/ l = [] /\ f = [].
 Proof.
   intros. functional induction @split A n l; cbn; inv H.
@@ -142,7 +137,7 @@ Lemma div2_inv :
 Proof.
   intros. destruct n.
     trivial.
-    assert (H' := div2_inv_aux (S n) ltac:(inv 1)).
+    assert (H' := @div2_inv_aux (S n) ltac:(inv 1)).
       contradiction.
 Qed.
 
@@ -150,39 +145,83 @@ Qed.
 Definition isDeque {A : Type} (d : Deque A) : Prop :=
   let '(f, r) := d in 2 <= length f + length r -> f <> [] /\ r <> [].
 
+Inductive isDeque' {A : Type} : Deque A -> Prop :=
+    | isDeque0 : isDeque' ([], [])
+    | isDeque1f : forall x : A, isDeque' ([x], [])
+    | isDeque1r : forall x : A, isDeque' ([], [x])
+    | isDequeSS :
+        forall (hf hr : A) (tf tr : list A),
+          isDeque' (hf :: tf, hr :: tr).
+
+Hint Constructors isDeque'.
+
 Lemma empty_isDeque :
   forall A : Type, isDeque (@empty A).
 Proof.
   cbn. inv 1.
 Qed.
 
+Lemma rev_cons :
+  forall (A : Type) (h : A) (t : list A),
+    exists (h' : A) (t' : list A), rev (h :: t) = h' :: t'.
+Proof.
+  cbn. intros. destruct (rev t).
+    exists h, []. cbn. reflexivity.
+    exists a, (l ++ [h]). cbn. reflexivity.
+Qed.
+
+Lemma isEmpty_rev_l :
+  forall (A : Type) (f r : list A),
+    isEmpty (rev f, r) = isEmpty (f, r).
+Proof.
+  destruct f, r; cbn; try destruct (rev f); cbn; reflexivity.
+Qed.
+
+Lemma isEmpty_rev_r :
+  forall (A : Type) (f r : list A),
+    isEmpty (f, rev r) = isEmpty (f, r).
+Proof.
+  destruct f, r; cbn; try destruct (rev r); cbn; reflexivity.
+Qed.
+
+Ltac rev_cons_aux h t := 
+  let h' := fresh "h'" in
+  let t' := fresh "t'" in
+  let H := fresh "H" in
+    destruct (rev_cons h t) as [h' [t' H]]; rewrite H.
+
+Ltac aux :=
+repeat match goal with
+    | H : halve _ = ([], _) |- _ =>
+        destruct (split_inv_l H); cbn in *
+    | H : halve _ = (_, []) |- _ =>
+        destruct (split_inv_r H); cbn in *
+    | H : S (S ?x) <= S (div2 ?x) |- _ =>
+        apply div2_inv in H; cbn in H; inv H
+    | |- context [rev (?h :: ?t)] => rev_cons_aux h t
+    | H : isEmpty (rev _, _) = _ |- _ =>
+        rewrite isEmpty_rev_l in H; cbn in H; try congruence
+    | H : isEmpty (_, rev _) = _ |- _ =>
+        rewrite isEmpty_rev_r in H; cbn in H; try congruence
+    | H : _ /\ _ |- _ => destruct H
+end; firstorder (auto; try congruence).
+
 Lemma deque_isDeque :
   forall (A : Type) (f r : list A), isDeque (deque f r).
 Proof.
-  intros. functional induction @deque A f r; cbn; intros; try omega.
-    destruct f0.
-      destruct (split_inv_r _ _ _ _ e1).
-        apply div2_inv in H0. destruct r; inv H0.
-        destruct H0; subst; cbn in *. contradiction.
-      destruct r0.
-        apply split_inv_l in e1. destruct e1.
-          destruct r as [| h1 [| h2 t]]; cbn in *; firstorder.
-          inv H0.
-        case_eq (rev (a :: f0)); intros.
-          cbn in H0. apply app_eq_nil in H0. inv H0.
-          split; congruence.
-    destruct f0.
-      destruct (split_inv_l _ _ _ _ e1).
-        destruct f as [| h1 [| h2 t]]; cbn in *; firstorder.
-        inv H0.
-      destruct r0.
-        apply split_inv_r in e1. destruct e1.
-          apply div2_inv in H0.
-            destruct f as [| h1 [| h2 t]]; cbn in *; firstorder.
-          inv H0.
-        case_eq (rev (a0 :: r0)); intros.
-          cbn in H0. apply app_eq_nil in H0. inv H0.
-          split; congruence.
+  intros. functional induction @deque A f r; cbn; intros.
+    destruct f0, r0; aux.
+    destruct f0, r0; aux.
+    destruct f as [| hf1 [| hf2 tf]], r as [| hr1 [| hr2 tr]]; cbn in *;
+      firstorder.
+Qed.
+
+Lemma deque_isDeque' :
+  forall (A : Type) (f r : list A), isDeque' (deque f r).
+Proof.
+  intros. functional induction @deque A f r; cbn; intros.
+    destruct f0, r0; aux.
+    destruct f0, r0; aux.
     destruct f as [| hf1 [| hf2 tf]], r as [| hr1 [| hr2 tr]]; cbn in *;
       firstorder.
 Qed.
@@ -198,8 +237,8 @@ Lemma tail_isDeque :
     tail d = Some d' -> isDeque d'.
 Proof.
   intros. functional induction @tail A d; inv H.
-    apply empty_isDeque.
     apply deque_isDeque.
+    apply empty_isDeque.
 Qed.
 
 Lemma snoc_isDeque :
@@ -213,39 +252,62 @@ Lemma init_isDeque :
     init d = Some d' -> isDeque d'.
 Proof.
   intros. functional induction @init A d; inv H.
-    apply empty_isDeque.
     apply deque_isDeque.
+    apply empty_isDeque.
 Qed.
 
 (* Properties of [isEmpty]. *)
+
 Lemma isEmpty_deque :
   forall (A : Type) (f r : list A),
     isEmpty (deque f r) = true -> f = [] /\ r = [].
 Proof.
   intros. functional induction @deque A f r;
-  cbn in *; auto; try congruence.
-    destruct f0.
-      destruct (split_inv_r _ _ _ _ e1).
-        apply div2_inv in H0. destruct r; inv H0.
-        tauto.
-      case_eq (rev (a :: f0)); intros.
-        cbn in H0. apply app_eq_nil in H0. destruct H0. congruence.
-        rewrite H0 in H. congruence.
-    destruct f0.
-      destruct (split_inv_l _ _ _ _ e1).
-        destruct f as [| h1 [| h2 t]]; cbn in *; firstorder.
-        inv H0.
-      congruence.
+  cbn; auto; try congruence.
+    destruct f0; aux.
+    destruct f0; aux.
     destruct f as [| h1 [| h2 t]], r; firstorder.
+Qed.
+
+(** TODO: port this to Deque.v *)
+Lemma isEmpty_deque' :
+  forall (A : Type) (f r : list A),
+    isEmpty (deque f r) =
+    match f, r with
+        | [], [] => true
+        | _, _ => false
+    end.
+Proof.
+  intros. functional induction @deque A f r.
+    destruct f0; aux.
+    destruct f0; aux.
+    destruct f as [| h1 [| h2 t]], r; firstorder.
+Qed.
+
+Lemma isEmpty_deque_true :
+  forall A : Type,
+    isEmpty (@deque A [] []) = true.
+Proof. cbn. reflexivity. Qed.
+
+Lemma isEmpty_deque_false_f :
+  forall (A : Type) (x : A) (f r : list A),
+    isEmpty (deque (x :: f) r) = false.
+Proof.
+  intros. rewrite isEmpty_deque'. reflexivity.
+Qed.
+
+Lemma isEmpty_deque_false_r :
+  forall (A : Type) (x : A) (f r : list A),
+    isEmpty (deque f (x :: r)) = false.
+Proof.
+  intros. rewrite isEmpty_deque'. destruct f; reflexivity.
 Qed.
 
 Lemma isEmpty_cons :
   forall (A : Type) (x : A) (d : Deque A),
     isEmpty (cons x d) = false.
 Proof.
-  destruct d as [f r]. unfold cons.
-  case_eq (isEmpty (deque (x :: f) r)); intros.
-    apply isEmpty_deque in H. inv H. congruence.
+  destruct d as [f r]. unfold cons. rewrite isEmpty_deque'. reflexivity.
 Qed.
 
 Lemma isEmpty_head_false :
@@ -280,9 +342,7 @@ Lemma isEmpty_snoc :
   forall (A : Type) (x : A) (d : Deque A),
     isEmpty (snoc x d) = false.
 Proof.
-  destruct d as [f r]. unfold snoc.
-  case_eq (isEmpty (deque f (x :: r))); intros.
-    apply isEmpty_deque in H. inv H. congruence.
+  destruct d as [f r]. unfold snoc. rewrite isEmpty_deque_false_r. auto.
 Qed.
 
 Lemma isEmpty_last_false :
@@ -312,8 +372,8 @@ Lemma isEmpty_init_true :
     init d = Some d' -> isEmpty d = false.
 Proof.
   intros. destruct d. functional inversion H; subst; cbn.
-    reflexivity.
     destruct l; reflexivity.
+    reflexivity.
 Qed.
 
 (* [size] and it's properties *)
@@ -324,26 +384,29 @@ Lemma size_empty :
   forall A : Type, size (@empty A) = 0.
 Proof. reflexivity. Qed.
 
+(** TODO: port to Deque.v *)
+Lemma split_length :
+  forall (A : Type) (n : nat) (l l1 l2 : list A),
+    split n l = (l1, l2) -> length l = length l1 + length l2.
+Proof.
+  intros. remember (l1, l2) as p.
+  functional induction @split A n l; inv H; inv H0.
+  cbn. erewrite IHp0; eauto.
+Qed.
+
 Lemma size_deque :
   forall (A : Type) (f r : list A),
     size (deque f r) = length f + length r.
 Proof.
-  intros. functional induction @deque A f r; cbn; try congruence.
-    unfold halve in e1. clear y.
-      functional induction @split A (Nat.div2 (length r)) r; inv e1; cbn.
-        rewrite rev_length, <- plus_n_O. reflexivity.
-        specialize (IHp _ _ e2). omega.
-    unfold halve in e1. clear y.
-      functional induction @split A (Nat.div2 (length f)) f; inv e1; cbn.
-        rewrite <- plus_n_O. apply rev_length.
-        specialize (IHp _ _ e2). omega.
+  intros. functional induction @deque A f r; cbn; auto;
+  apply split_length in e1; cbn in e1; rewrite rev_length; omega.
 Qed.
 
 Lemma size_cons :
   forall (A : Type) (x : A) (d : Deque A),
     size (cons x d) = S (size d).
 Proof.
-  intros. unfold cons. destruct d. rewrite size_deque. cbn. reflexivity.
+  destruct d as [f r]. unfold cons. rewrite size_deque. cbn. reflexivity.
 Qed.
 
 Lemma size_tail :
@@ -351,8 +414,8 @@ Lemma size_tail :
     tail d = Some d' -> size d' = pred (size d).
 Proof.
   intros. functional inversion H; subst.
-    reflexivity.
     rewrite size_deque. cbn. reflexivity.
+    reflexivity.
 Qed.
 
 Lemma size_snoc :
@@ -367,8 +430,8 @@ Lemma size_init :
     init d = Some d' -> size d' = pred (size d).
 Proof.
   intros. functional inversion H; subst.
-    reflexivity.
     rewrite size_deque. cbn. omega.
+    reflexivity.
 Qed.
 
 (* [map] and its properties *)
@@ -393,20 +456,11 @@ Lemma fmap_deque :
   forall (A B : Type) (g : A -> B) (f r : list A),
     fmap g (deque f r) = deque (map g f) (map g r).
 Proof.
-  intros. functional induction @deque A f r; cbn;
-  auto; unfold halve in *.
-    rewrite ?map_length, map_split'. destruct r as [| h1 [| h2 t]]; cbn.
-      contradiction.
-      contradiction.
-      cbn in *. destruct (split (Nat.div2 (length t)) (h2 :: t)).
-        inv e1. cbn. rewrite map_rev. reflexivity.
-    destruct f as [| h1 [| h2 t]].
-      contradiction.
-      contradiction.
-      cbn in *. change (g h2 :: map g t) with (map g (h2 :: t)).
-        rewrite ?map_length, map_split'.
-        destruct (split (Nat.div2 (length t)) (h2 :: t)).
-        inv e1. cbn. rewrite map_rev. reflexivity.
+  intros. functional induction @deque A f r; unfold deque, halve.
+    rewrite ?map_split', ?map_length. cbn in *. rewrite e1, map_rev.
+      cbn. reflexivity.
+    rewrite ?map_split', ?map_length. cbn in *. rewrite e1, map_rev.
+      cbn. reflexivity.
     destruct f as [| hf1 [| hf2 tf]], r as [| hr1 [| hr2 tr]]; cbn;
     firstorder.
 Qed.
@@ -427,7 +481,7 @@ Lemma fmap_head :
     end.
 Proof.
   intros. functional induction @head A d; cbn; try reflexivity.
-  destruct _x as [| h1 [| h2 t]]; cbn; tauto.
+  destruct _x as [| h1 [| h2 t]]; cbn; try tauto.
 Qed.
 
 Lemma fmap_tail :
@@ -500,10 +554,8 @@ Lemma head_cons :
     head (cons x d) = Some x.
 Proof.
   destruct d as [f r]. unfold cons. remember (x :: f) as f'.
-  functional induction @deque A f' r; cbn; try congruence.
-  destruct f as [| hf tf]; cbn in *.
-    inv e1.
-    destruct (split (div2 (length tf)) (hf :: tf)). inv e1.
+  functional induction @deque A f' r; cbn in *; try congruence.
+  destruct (split (div2 (length _x1)) (_x0 :: _x1)). inv e1.
 Qed.
 
 Lemma head_snoc :
@@ -512,29 +564,26 @@ Lemma head_snoc :
 Proof.
   destruct d as [f r]. unfold snoc. remember (x :: r) as r'. intros.
   functional induction @deque A f r'; cbn in *; try inv Heqr'; try congruence.
-    2: destruct _x, r; firstorder.
-    destruct r as [| h1 [| h2 t]]; cbn in *.
-      congruence.
+    destruct _x1 as [| h1 [| h2 t]]; cbn in *.
       inv e1.
+      destruct H; firstorder.
       destruct (H ltac:(omega)). congruence.
+    destruct _x, r; firstorder.
 Qed.
 
 (* [toList] and its properties. *)
 Definition toList {A : Type} (d : Deque A) : list A :=
   let '(f, r) := d in f ++ rev r.
 
+(** TODO: port to Deque.v *)
 Lemma toList_deque :
   forall (A : Type) (f r : list A),
     toList (deque f r) = f ++ rev r.
 Proof.
   intros. functional induction @deque A f r; cbn; auto;
-  unfold halve in *.
-    clear y. functional induction @split A (Nat.div2 (length r)) r; inv e1; cbn.
-      apply app_nil_r.
-      rewrite app_assoc, (IHp _ _ e2). reflexivity.
-    clear y. functional induction @split A (Nat.div2 (length f)) f; inv e1; cbn.
-      rewrite rev_involutive, app_nil_r. reflexivity.
-      rewrite (IHp _ _ e2). reflexivity.
+  unfold halve in *; apply split_spec in e1.
+    rewrite <- rev_app_distr, <- e1. reflexivity.
+    rewrite rev_involutive, app_nil_r, e1. reflexivity.
 Qed.
 
 Lemma toList_empty :
@@ -557,11 +606,9 @@ Lemma toList_head :
         | h :: _ => Some h
     end.
 Proof.
-  intros. functional induction @head A d; cbn; auto.
-  cbn in H. destruct _x as [| h1 [| h2 t]]; cbn; try tauto.
-  cbn in *. destruct H.
-    omega.
-    contradiction.
+  intros. functional induction @head A d; cbn in *; auto.
+  destruct _x as [| h1 [| h2 t]]; cbn in *; try tauto.
+  destruct (H ltac:(omega)). congruence.
 Qed.
 
 Lemma toList_tail :
@@ -593,10 +640,10 @@ Lemma toList_last :
     end.
 Proof.
   intros. functional induction @last A d; cbn; auto.
-    cbn in H. destruct _x as [| h1 [| h2 t]]; cbn; try tauto.
-      cbn in *. destruct H. omega. contradiction.
     case_eq (rev (_x ++ rev _x0 ++ [x])); intros;
       rewrite !rev_app_distr in H0; cbn in *; congruence.
+    cbn in H. destruct _x as [| h1 [| h2 t]]; cbn; try tauto.
+      cbn in *. destruct (H ltac:(omega)). contradiction.
 Qed.
 
 Lemma toList_init :
@@ -635,9 +682,6 @@ Lemma drev_inv :
   forall (A : Type) (d : Deque A), drev (drev d) = d.
 Proof. destruct d; reflexivity. Qed.
 
-Compute drev (deque [1] [2; 3]).
-Compute deque [1; 2] [].
-
 Lemma drev_deque_toList :
   forall (A : Type) (f r : list A),
     toList (drev (deque f r)) = toList (deque r f).
@@ -652,12 +696,12 @@ Lemma drev_deque :
 Proof.
   intros. assert (isDeque (deque f r)) by apply deque_isDeque.
   functional induction @deque A f r; cbn; auto; unfold halve in *.
-    destruct r as [| hr1 [| hr2 tr]]; cbn in *; try contradiction.
-      case_eq (split (Nat.div2 (length tr)) (hr2 :: tr)); intros.
-        rewrite H0 in e1. inv e1.
-    destruct f as [| hf1 [| hf2 tf]]; cbn in *; try contradiction.
-      case_eq (split (Nat.div2 (length tf)) (hf2 :: tf)); intros.
-        rewrite H0 in e1. inv e1.
+    destruct _x1 as [| hr1 [| hr2 tr]]; cbn in *; inv e1.
+      case_eq (split (Nat.div2 (length tr)) (hr1 :: hr2 :: tr)); intros.
+        rewrite H0 in H1. inv H1.
+    destruct _x1 as [| hf1 [| hf2 tf]]; cbn in *; inv e1.
+      case_eq (split (Nat.div2 (length tf)) (hf1 :: hf2 :: tf)); intros.
+        rewrite H0 in H1. inv H1.
     destruct f as [| hf1 [| hf2 t]], r as [| hr1 [| hr2 tr]]; cbn; firstorder.
 Qed.
 
@@ -673,7 +717,7 @@ Lemma drev_head :
     head (drev d) = last d.
 Proof.
   intros. functional induction @head A d; cbn; auto.
-  destruct _x0, _x; reflexivity.
+    destruct _x0, _x; reflexivity.
 Qed.
 
 Lemma drev_tail :
@@ -685,9 +729,9 @@ Lemma drev_tail :
     end.
 Proof.
   intros. functional induction @tail A d; cbn; trivial.
-    destruct _x as [| h1 [| h2 t]]; try contradiction.
-      cbn in H. destruct (H ltac:(omega)). congruence.
     destruct r as [| hr1 [| hr2 [| hr3 tr]]], t; cbn; auto.
       destruct (split (Nat.div2 (length t)) (a :: t)).
         cbn. reflexivity.
+    destruct _x as [| h1 [| h2 t]]; cbn in *; firstorder.
+      destruct (H ltac:(omega)). congruence.
 Qed.
